\documentclass[12pt,a4paper]{article}
\usepackage[latin1]{inputenc}
\usepackage{amsmath}
\usepackage{amsfonts}
\usepackage{amssymb}
\usepackage{graphicx}
\usepackage{cancel}
\usepackage[left=2.00cm, right=2.00cm, top=2.00cm, bottom=2.00cm]{geometry}
\author{H.O.W.K.E}
\title{Kunci Ujian Matematika SMP Tahap 3 }
\begin{document}
	\maketitle
	\paragraph{LV 1}
	\begin{enumerate}
	\item $\dfrac{3^2\cdot 4^{-2} \cdot 5}{2^{-4}\cdot 3^3\cdot 25}=3^{2-3}\cdot(2^2)^{-2}\cdot2^4\cdot \dfrac{1}{5}=3^{-1}\cdot 2^{-4}\cdot 2^4 \cdot \dfrac{1}{5}
	=\dfrac{1}{3}\cdot 2^{-4+4}\cdot \dfrac{1}{5}=\dfrac{1}{3}\cdot\dfrac{1}{5}=\dfrac{1}{15}
	$
	\item $3^{-1}-3^{-3}=\dfrac{1}{3}-\dfrac{1}{27}=\dfrac{3-1}{27}=\dfrac{2}{27}$
	\item $(\dfrac{1}{13})^0(\dfrac{2}{3})^6(\dfrac{4}{9})^{-3}=(1)(\dfrac{2^6}{3^6})(\dfrac{9^3}{4^3})=\dfrac{2^6}{3^6}\cdot\dfrac{3^6}{2^6}=\dfrac{\cancelto{1}{2^6}}{\cancelto{1}{3^6}}\cdot\dfrac{\cancelto{1}{3^6}}{\cancelto{1}{2^6}}=1$
	\item $(\dfrac{2}{3})^{3}=\dfrac{8}{27}$
	\item $\dfrac{3}{3^{-2}}=3\cdot3^{2}=3^{1+2}=3^3=27$
	\end{enumerate}
	\paragraph{LV 2}
	\begin{enumerate}
		\item $\dfrac{x^2b^2c^2}{xbc^{-1}}=x^{2-1}b^{2-1}c^{2-(-1)}=xbc^3$
		\item $\dfrac{25u^{12}p^{24}q}{125up^{15}q^{16}}=\dfrac{1}{5}u^{12-1}p^{24-15}=\dfrac{1}{5}u^{11}p^9$
		\item $(\sqrt{{a^2}})^2\cdot\dfrac{1}{a^{-1}}=a^2\cdot a=a^3$
		\item $\sqrt{-a^{2}-(-a)^{2}+{-a^2}}=\sqrt{-a^2-a^2-a^2}=\sqrt{-3a^2}=a\sqrt{-3}$
		\item $\dfrac{a^{-6}}{a^{-7}}=\dfrac{a^7}{a^6}=a^{7-6}=a$
	\end{enumerate}
	\paragraph{LV 3}
	\begin{enumerate}
			\item $\Big(\dfrac{a^{4}b^{12}c^{4}}{a^{-10}b^{-5}c^{-4}}\Big)^{-\frac{1}{2}} = (a^{4-(-10)}b^{12-(-5)}c^{4-(-4)})^{-\frac{1}{2}}=(a^{14}b^{17}c^{8})^{-\frac{1}{2}}=a^{-7}b^{-\frac{17}{2}}c^{-4}=\dfrac{1}{a^7\sqrt{b^{17}}c^{4}}$
			\item $\Big(\dfrac{x^{-14}\sqrt[12]{x^{4}}x^{8}}{x^{-8}x^{-1/5}x^{-1/4}}\Big)^{-\frac{1}{2}} 
			=(x^{(-14+\frac{4}{12}+8)-(-8+(-\frac{1}{5})+(-\frac{1}{4}))})^{\frac{1}{2}x^{\frac{167}{60}\cdot\frac{1}{2}}=x^{\frac{167}{120}}$
			\item $ \Big(\sqrt{a}\cdot\sqrt{a^4}\Big)^{-2}=a^{(\frac{1}{2}+2)\cdot\frac{1}{2}}=a^{2\frac{1}{2}}$
			\item $((a^2)^{16})^{17}=a^{544}$
			\item $p^{1/2}p^{0}p^{1/4}=p^{\frac{1}{2}+0+\frac{1}{4}}=p^{\frac{3}{4}}$
	\end{enumerate}
	\paragraph{LV 4}
	\begin{enumerate}
			\item $\big(625z^{\frac{2}{8}}f^{\frac{1}{4}}\big)^{\frac{1}{2}}=25z^{\frac{1}{8}}f^{\frac{1}{8}}$
			\item $(\sqrt[14]{x^7})^7=x^{\frac{7}{2}}$
			\item $\sqrt{p}^{\sqrt{2}} \cdot \sqrt{p}^{3\sqrt{2}}=\sqrt{p}^{\sqrt{2}+3\sqrt{2}}=\sqrt{p}^{4\sqrt{2}}$
			\item $\sqrt{\sqrt{\sqrt{\sqrt{\sqrt{\dfrac{1}{2}}}}}}=\dfrac{1}{2^\frac{1}{5}}$
			\item $\dfrac{z^\pi\cdot z^{2\pi}}{z^{3\pi}}=z^{(\pi+2\pi-3\pi)}=z^0=1PENGUMU$
	\end{enumerate}
	
	
\end{document}